Added Telemetry Decoder example for BRASS.

src/Examples/Tutorial/NotInList.v
@@ -1,9 +1,30 @@
-Require Import Tutorial.
+Require Import Coq.Strings.Ascii
+        Coq.Bool.Bool
+        Coq.Lists.List.
+
+Require Export Coq.Vectors.Vector
+        Coq.omega.Omega
+        Coq.Strings.Ascii
+        Coq.Bool.Bool
+        Coq.Bool.Bvector
+        Coq.Lists.List.
+
+Require Import Fiat.ADT
+        Fiat.ADTRefinement.GeneralBuildADTRefinements.
 
 
 (* A specification of what it means to choose a number that is not in a particular list *)
 Definition notInList (ls : list nat) :=
   {n : nat | ~In n ls}%comp.
+
+Ltac refines := intros; repeat computes_to_econstructor; repeat computes_to_inv; subst.
+Ltac arithmetic := intros;
+  repeat match goal with
+         | [ |- context[max ?a ?b] ] => let Heq := fresh "Heq" in
+                                        destruct (Max.max_spec a b) as [ [? Heq] | [? Heq] ];
+                                          rewrite Heq in *; clear Heq
+         end; omega.
+
 
 (* We can use a simple property to justify a decomposition of the original spec. *)
 Theorem notInList_decompose : forall ls,
@@ -43,7 +64,13 @@ Proof.
   arithmetic.
 Qed.
 
+Ltac begin := eexists; intro; set_evars.
+
+Ltac monad_simpl := autosetoid_rewrite with refine_monad;
+                   try simplify_with_applied_monad_laws; simpl.
+
 (* Let's derive an efficient implementation. *)
+
 Theorem implementation : { f : list nat -> Comp nat | forall ls, refine (notInList ls) (f ls) }.
 Proof.
   begin.
@@ -55,7 +82,7 @@ Proof.
 Defined.
 
 (* We can extract the program that we found as a standlone, executable Gallina term. *)
-Definition impl := Eval simpl in projT1 implementation.
+Definition impl := Eval simpl in proj1_sig implementation.
 Print impl.
 
 Eval compute in impl (1 :: 7 :: 8 :: 2 :: 13 :: 6 :: nil).
