src/Narcissus/Formats/StringOpt.v
@@ -91,4 +91,133 @@ Section String.
       }
     }
   Qed.
+
+  Definition decode_string_with_term_char
+           (term_char : Ascii.ascii)
+           (b : B) (cd : CacheDecode)
+    : option (string * B * CacheDecode).
+    refine (Fix well_founded_lt_b
+           (fun _ => CacheDecode -> option (string * B * CacheDecode))
+      (fun b rec cd =>
+         (`(a, b1, e1) <- Decode_w_Measure_lt decode_ascii b cd _;
+      If ascii_dec a term_char Then
+        Some (EmptyString, proj1_sig b1, e1)
+      Else
+      (`(xs, b2, e2) <- rec _ (proj2_sig b1) e1;
+      Some (String a xs, b2, e2)))) b cd).
+    exact ascii_decode_lt.
+  Defined.
+
+  Definition format_string_with_term_char
+             (term_char : Ascii.ascii)
+             (xs : string) (ce : CacheFormat)
+    : Comp (B * CacheFormat) :=
+    format_string (xs ++ (String term_char EmptyString)) ce.
+
+  Theorem String_decode_with_term_char_correct
+          {P : CacheDecode -> Prop}
+    : forall term_char (P_OK : cache_inv_Property P (fun P => forall b cd, P cd -> P (addD cd b))),
+      CorrectDecoder
+        monoid
+        (fun s => forall s1 s2, s <> s1 ++ String term_char s2)%string
+        (fun _ _ => True)
+        (format_string_with_term_char term_char)
+        (decode_string_with_term_char term_char) P.
+  Proof.
+    split.
+    { intros env env' xenv s s' ext ? Eeq Ppred Ppred_rest Penc.
+      subst.
+      generalize dependent env.
+      revert env' xenv s' env_OK.
+      induction s.
+      { intros.
+        unfold format_string_with_term_char in Penc.
+        unfold decode_string_with_term_char.
+        simpl in Penc; unfold Bind2 in *; computes_to_inv; subst; simpl in *.
+        rewrite mempty_right in Penc''; inversion Penc''; subst.
+        destruct v; simpl in *.
+        eapply Ascii_decode_correct in Penc; eauto.
+        destruct Penc; intuition.
+        eexists; rewrite Init.Wf.Fix_eq.
+        eapply Decode_w_Measure_lt_eq in H0; destruct_ex.
+        rewrite H0; simpl.
+        destruct (ascii_dec term_char term_char); simpl; try congruence.
+        eauto.
+        intros.
+        repeat (apply functional_extensionality; intros; f_equal).
+        rewrite H1; reflexivity.
+      }
+      { intros.
+        unfold format_string_with_term_char in Penc;
+          unfold decode_string_with_term_char.
+        simpl in *.
+        unfold Bind2 in *; computes_to_inv; subst.
+        injection Penc''; intros; subst.
+        destruct v; destruct v0.
+        destruct (proj1 (Ascii_decode_correct P_OK) _ _ _ _ _ (mappend b0 ext) env_OK Eeq I I Penc) as [? [? [? xenv_OK] ] ].
+      simpl.
+      unfold format_string_with_term_char in IHs.
+      simpl in Penc'; eapply IHs in Penc'.
+      destruct Penc'; intuition.
+      eexists; rewrite Init.Wf.Fix_eq.
+      eapply Decode_w_Measure_lt_eq in H; destruct_ex.
+      rewrite <- mappend_assoc, H; simpl.
+      destruct (ascii_dec a term_char); simpl.
+      - elimtype False.
+        subst; eapply (Ppred "")%string; simpl; reflexivity.
+      - intuition.
+        unfold decode_string_with_term_char in H2.
+        rewrite H2; simpl; eauto.
+        eauto.
+        eauto.
+      - intros; repeat (apply functional_extensionality; intros; f_equal).
+        rewrite H3; reflexivity.
+      - unfold not; intros; eapply (Ppred (String a s1) s2); simpl; congruence.
+      - eauto.
+      - eauto.
+      }
+    }
+    { unfold decode_string_with_term_char, format_string_with_term_char;
+        intros env env' xenv' data bin;
+        revert env env' xenv' data.
+      eapply (@well_founded_induction _ _ well_founded_lt_b) with
+      (a := bin); intros.
+      rewrite Coq.Init.Wf.Fix_eq in H2; auto; simpl.
+      apply DecodeBindOpt2_inv in H2;
+        destruct H2 as [? [? [? [? ?] ] ] ]; injections; subst.
+      destruct (decode_ascii x env') as [ [ [? ?] ?] | ] eqn: ? .
+      - destruct (Decode_w_Measure_lt_eq _ _ _ ascii_decode_lt Heqo).
+        rewrite H4 in H2; injections.
+        destruct (ascii_dec x0 term_char) eqn: ?; simpl in H3.
+        + injections.
+          eapply (proj2 (Ascii_decode_correct P_OK)) in Heqo; eauto;
+            destruct Heqo as [? [? ?] ]; destruct_ex; intuition; subst.
+          simpl.
+          eexists _, _; intuition.
+          computes_to_econstructor; eauto.
+          computes_to_econstructor; eauto.
+          simpl; rewrite mempty_right; eauto.
+          destruct s1; simpl in *; discriminate.
+          eauto.
+        + eapply (proj2 (Ascii_decode_correct P_OK)) in Heqo; eauto;
+            destruct Heqo as [? [? ?] ]; destruct_ex.
+          symmetry in H3; apply DecodeBindOpt2_inv in H3;
+            destruct H3 as [? [? [? [? ?] ] ] ]; injections; subst.
+          eapply H in H3; intuition.
+          destruct_ex; intuition; subst; eauto.
+          eexists _, _; intuition.
+          simpl.
+          computes_to_econstructor; eauto.
+          computes_to_econstructor; eauto.
+          simpl; rewrite mappend_assoc; eauto.
+          destruct s1; simpl in *; injections; intros; congruence.
+          simpl; eauto.
+          simpl; eauto.
+      - eapply Decode_w_Measure_lt_eq' in Heqo; rewrite Heqo in H2;
+          discriminate.
+      - intros; repeat (apply functional_extensionality; intros; f_equal).
+        rewrite H3; reflexivity.
+    }
+  Qed.
+
 End String.
