src/CertifiedExtraction/Benchmarks/MicroEncodersSetup.v
@@ -1,10 +1,10 @@
 Require Export
-        Fiat.BinEncoders.Env.Automation.Solver
-        Fiat.BinEncoders.Env.Common.Specs
-        Fiat.BinEncoders.Env.Common.Compose
-        Fiat.BinEncoders.Env.BinLib.Core
-        Fiat.BinEncoders.Env.Lib.FixList
-        Fiat.BinEncoders.Env.BinLib.FixInt.
+        Fiat.Narcissus.Automation.Solver
+        Fiat.Narcissus.Common.Specs
+        Fiat.Narcissus.Common.Compose
+        Fiat.Narcissus.BinLib.Core
+        Fiat.Narcissus.Lib.FixList
+        Fiat.Narcissus.BinLib.FixInt.
 
 Require Export
         Fiat.CertifiedExtraction.RemoveSkips
@@ -21,27 +21,27 @@ Require Export
         Fiat.Common.BoundedLookup
         Fiat.Common.ilist
         Fiat.Computation
-        Fiat.BinEncoders.Env.Automation.SolverOpt
-        Fiat.BinEncoders.Env.BinLib.Bool
-        Fiat.BinEncoders.Env.BinLib.Core
-        Fiat.BinEncoders.Env.BinLib.Enum
-        Fiat.BinEncoders.Env.BinLib.FixInt
-        Fiat.BinEncoders.Env.Common.Compose
-        Fiat.BinEncoders.Env.Common.ComposeCheckSum
-        Fiat.BinEncoders.Env.Common.ComposeIf
-        Fiat.BinEncoders.Env.Common.Specs
-        Fiat.BinEncoders.Env.Common.WordFacts
-        Fiat.BinEncoders.Env.Lib.FixList
-        Fiat.BinEncoders.Env.Lib.IList
-        Fiat.BinEncoders.Env.Lib2.Bool
-        Fiat.BinEncoders.Env.Lib2.EnumOpt
-        Fiat.BinEncoders.Env.Lib2.FixListOpt
-        Fiat.BinEncoders.Env.Lib2.NatOpt
-        Fiat.BinEncoders.Env.Lib2.NoCache
-        Fiat.BinEncoders.Env.Lib2.SumTypeOpt
-        Fiat.BinEncoders.Env.Lib2.Vector
-        Fiat.BinEncoders.Env.Lib2.WordOpt
-        Fiat.BinEncoders.Env.Lib2.IPChecksum.
+        Fiat.Narcissus.Automation.SolverOpt
+        Fiat.Narcissus.BinLib.Bool
+        Fiat.Narcissus.BinLib.Core
+        Fiat.Narcissus.BinLib.Enum
+        Fiat.Narcissus.BinLib.FixInt
+        Fiat.Narcissus.Common.Compose
+        Fiat.Narcissus.Common.ComposeCheckSum
+        Fiat.Narcissus.Common.ComposeIf
+        Fiat.Narcissus.Common.Specs
+        Fiat.Narcissus.Common.WordFacts
+        Fiat.Narcissus.Lib.FixList
+        Fiat.Narcissus.Lib.IList
+        Fiat.Narcissus.Lib2.Bool
+        Fiat.Narcissus.Lib2.EnumOpt
+        Fiat.Narcissus.Lib2.FixListOpt
+        Fiat.Narcissus.Lib2.NatOpt
+        Fiat.Narcissus.Lib2.NoCache
+        Fiat.Narcissus.Lib2.SumTypeOpt
+        Fiat.Narcissus.Lib2.Vector
+        Fiat.Narcissus.Lib2.WordOpt
+        Fiat.Narcissus.Lib2.IPChecksum.
 
 Open Scope binencoders_scope.
 
