src/Narcissus/Examples/BRASS/Telemetry.v
@@ -1,0 +1,242 @@
+Require Import
+        Coq.Strings.String
+        Coq.Vectors.Vector.
+
+Require Import
+        Fiat.Common.SumType
+        Fiat.Common.BoundedLookup
+        Fiat.Common.ilist
+        Fiat.Computation
+        Fiat.QueryStructure.Specification.Representation.Notations
+        Fiat.QueryStructure.Specification.Representation.Heading
+        Fiat.QueryStructure.Specification.Representation.Tuple
+        Fiat.Narcissus.BinLib.Core
+        Fiat.Narcissus.Common.Specs
+        Fiat.Narcissus.Common.ComposeOpt
+        Fiat.Narcissus.Automation.Solver
+        Fiat.Narcissus.Formats.StringOpt.
+
+Require Import
+        Coq.NArith.NArith
+        Recdef.
+
+Require Import Bedrock.Word.
+
+Import Vectors.VectorDef.VectorNotations.
+Open Scope string_scope.
+Open Scope Tuple_scope.
+
+(* Start Example Derivation. *)
+
+Section Coordinate_Decoder.
+
+Definition Coordinate :=
+  @Tuple <"Time" :: N,
+          "Latitude" :: Z * N,
+          "Longitude" :: Z * N >.
+
+Function N_to_string' (n : N) {wf N.lt n}: string :=
+  match n with
+  | N0 => EmptyString
+  | _ => String.append (N_to_string' (BinNatDef.N.div n 10))%N (String (Ascii.ascii_of_N (48 + BinNatDef.N.modulo n 10))%N EmptyString)
+end.
+intros; apply N.div_lt; reflexivity.
+apply N.lt_wf_0.
+Defined.
+
+Definition N_to_string (n : N) :=
+  match n with
+  | N0 => "0"
+  | _ => N_to_string' n
+  end.
+
+Goal (N_to_string 10 ="10")%N%string.
+  unfold N_to_string;
+  repeat first [reflexivity
+               | rewrite N_to_string'_equation; simpl].
+Qed.
+
+Goal (N_to_string 1030 ="1030")%N%string.
+  unfold N_to_string;
+  repeat first [reflexivity
+               | rewrite N_to_string'_equation; simpl].
+Qed.
+
+Fixpoint string_to_N (s : string) : N :=
+  match s with
+  | EmptyString => 0
+  | String c s' => ((Ascii.N_of_ascii c - 48) * 10^(N.of_nat (String.length s'))) + (string_to_N s')
+  end%N.
+
+Goal (10 = string_to_N "10")%N%string.
+  reflexivity.
+Qed.
+
+Goal (1030 = string_to_N "1030")%N%string.
+  reflexivity.
+Qed.
+
+Goal (0 = string_to_N "0")%N%string.
+  reflexivity.
+Qed.
+
+Lemma string_length_append :
+  forall s s', (String.length (s ++ s') = String.length s + String.length s')%nat.
+Proof.
+  induction s; simpl; intros; eauto.
+Qed.
+
+Lemma N_of_nat_distr :
+  forall n n' : nat, (N.of_nat (n + n') = N.of_nat n + N.of_nat n')%N.
+Proof.
+  induction n; intros; eauto.
+  simpl plus.
+  rewrite !Nat2N.inj_succ, IHn, N.add_succ_l; reflexivity.
+Qed.
+
+Lemma string_to_N_append : forall s s',
+    (string_to_N (s ++ s') = (string_to_N s * 10^(N.of_nat (String.length s'))) +
+                             (string_to_N s'))%N.
+Proof.
+  induction s; simpl; intros; eauto.
+  rewrite IHs.
+  rewrite !N.add_assoc, string_length_append,
+  N_of_nat_distr, N.pow_add_r, N.mul_add_distr_r, N.mul_assoc.
+  reflexivity.
+Qed.
+
+Lemma N_to_string_inv
+  : forall n, string_to_N (N_to_string n) = n.
+Proof.
+  destruct n; simpl.
+  - reflexivity.
+  - pattern (N.pos p), (N_to_string' (N.pos p)).
+    apply N_to_string'_ind; intros; eauto.
+    subst.
+    rewrite string_to_N_append.
+    rewrite H.
+    simpl String.length; simpl N.of_nat.
+    unfold string_to_N.
+    rewrite Ascii.N_ascii_embedding.
+    rewrite (N.div_mod' _x 10) at 3.
+    simpl N.of_nat.
+    replace (10 ^ 1)%N with 10%N by reflexivity.
+    rewrite N.mul_comm.
+    f_equal.
+    generalize (_x mod 10)%N; intro.
+    rewrite (Nplus_comm 48), (N.add_sub n), N.mul_1_r, N.add_0_r; reflexivity.
+    eapply (N.add_lt_mono_l _ 208 48).
+    etransitivity.
+    eapply N.mod_bound_pos.
+    eapply N.le_0_l.
+    reflexivity.
+    reflexivity.
+Qed.
+
+Definition string_to_Z (s : string) : Z :=
+  match s with
+  | String "-" s' => BinInt.Z.mul (BinInt.Z.of_N (string_to_N s')) (-1)
+  | _ => BinInt.Z.of_N (string_to_N s)
+  end.
+
+Definition Z_to_string (z : Z) : string :=
+  match z with
+  | Zneg _ => String "-" (N_to_string (BinIntDef.Z.abs_N z))
+  | _ => (N_to_string (BinIntDef.Z.abs_N z))
+  end.
+
+Lemma Z_to_string_inv
+  : forall z, string_to_Z (Z_to_string z) = z.
+Proof.
+  destruct z eqn: ?; simpl.
+  - reflexivity.
+  - unfold string_to_Z.
+    destruct (N_to_string' (N.pos p)) eqn: ?.
+Admitted.
+
+Definition Coordinate_format
+           (coords : Coordinate) :=
+          format_string_with_term_char " " (N_to_string (coords!"Time"))
+    ThenC format_string_with_term_char "." (Z_to_string (fst coords!"Latitude"))
+    ThenC format_string_with_term_char " " (N_to_string (snd coords!"Latitude"))
+    ThenC format_string_with_term_char "." (Z_to_string (fst coords!"Longitude"))
+    ThenC format_string_with_term_char " " (N_to_string (snd coords!"Longitude"))
+    DoneC.
+
+Definition Coordinate_decoder
+  : CorrectDecoderFor (fun _ => True) Coordinate_format.
+Proof.
+  start_synthesizing_decoder.
+  normalize_compose monoid.
+  decode_step idtac.
+  intros; eapply String_decode_with_term_char_correct.
+  decode_step idtac.
+  admit.
+  decode_step idtac.
+  decode_step idtac.
+  intros; eapply String_decode_with_term_char_correct.
+  decode_step idtac.
+  admit.
+  decode_step idtac.
+  decode_step idtac.
+  intros; eapply String_decode_with_term_char_correct.
+  decode_step idtac.
+  admit.
+  decode_step idtac.
+  decode_step idtac.
+  intros; eapply String_decode_with_term_char_correct.
+  decode_step idtac.
+  admit.
+  decode_step idtac.
+  decode_step idtac.
+  intros; eapply String_decode_with_term_char_correct.
+  decode_step idtac.
+  admit.
+  decode_step idtac.
+  simpl; intros **; eapply CorrectDecoderinish.
+  unfold Domain, GetAttribute, GetAttributeRaw in *; simpl in *;
+    (let a' := fresh in
+     intros a'; repeat destruct a' as [? a']; unfold Domain, GetAttribute, GetAttributeRaw in *; simpl in *; intros **; intuition;
+     repeat
+       match goal with
+       | H:_ = _
+         |- _ => first
+                   [ apply decompose_pair_eq in H; (let H1 := fresh in
+                                                    let H2 := fresh in
+                                                    destruct H as [H1 H2]; simpl in H1; simpl in H2)
+                   | rewrite H in * ]
+       end).
+  destruct prim_fst0, prim_fst1; simpl in *.
+  apply (f_equal string_to_N) in H7.
+  apply (f_equal string_to_N) in H9.
+  apply (f_equal string_to_N) in H11.
+  apply (f_equal string_to_Z) in H8.
+  apply (f_equal string_to_Z) in H10.
+  rewrite N_to_string_inv, Z_to_string_inv in *.
+  subst.
+  reflexivity.
+  unfold GetAttribute, GetAttributeRaw; simpl.
+  Print Ltac build_fully_determined_type.
+  decide_data_invariant.
+  apply (@decides_True' _ proj).
+  setoid_rewrite <- BoolFacts.string_dec_bool_true_iff;
+    split; intro H5; apply H5.
+  setoid_rewrite <- BoolFacts.string_dec_bool_true_iff;
+    split; intro H5; apply H5.
+  setoid_rewrite <- BoolFacts.string_dec_bool_true_iff;
+    split; intro H5; apply H5.
+  setoid_rewrite <- BoolFacts.string_dec_bool_true_iff;
+    split; intro H5; apply H5.
+  setoid_rewrite <- BoolFacts.string_dec_bool_true_iff;
+    split; intro H5; apply H5.
+  synthesize_cache_invariant.
+  repeat optimize_decoder_impl.
+
+Defined.
+
+Definition Coordinate_decoder_impl :=
+  Eval simpl in (fst (proj1_sig Coordinate_decoder)).
+
+End Coordinate_Decoder.
+
+Print Coordinate_decoder_impl.
