src/Narcissus/Formats/InternetChecksum.v
@@ -758,7 +758,7 @@ Proof.
   reflexivity.
 Qed.
 
-(* 8.7 Definition 
+(* 8.7 Definition *)
    Lemma wmsb_combine {sz} :
   forall (w : word (S sz)) b,
   exists w' : word sz,
@@ -777,8 +777,9 @@ Proof.
     eapply WS_match_eq_refl.
     rewrite Heq at 1.
     reflexivity.
-Qed. *)
+Qed.
 
+(*
 (* 8.4 Definition *)
    Lemma wmsb_combine {sz} :
   forall (w : word (S sz)) b,
@@ -798,7 +799,7 @@ Proof.
     eapply WS_match_eq_refl.
     rewrite Heq at 1.
     reflexivity.
-Qed. 
+Qed. *)
 
 Lemma normalizeZ_OneCToZ {sz} :
   forall w: word (S sz), normalizeZ sz (OneCToZ w) = (OneCToZ w).
@@ -807,7 +808,7 @@ Proof.
   apply normalizeZ_noop.
   unfold OneCToZ.
   pose proof (Npow2_ge_one sz).
-  (* 8.7 script: 
+  (* 8.7 script:  *)
      destruct (wmsb _ _) eqn:Heqb; destruct (wordToN _) eqn:Heqn;
     repeat match goal with
            | _ => lia
@@ -824,7 +825,7 @@ Proof.
                rewrite wordToN_combine in Heqn;
                pose proof (wordToN_bound w');
                simpl in Heqn; rewrite Heqb in Heqn; simpl in Heqn
-           end. *)
+           end. (*
   (* 8.4 script *)
   destruct (wmsb _ _) eqn:Heqb; destruct (wordToN _) eqn:Heqn;
     repeat match goal with
@@ -842,7 +843,7 @@ Proof.
                rewrite wordToN_combine in Heqn;
                pose proof (wordToN_bound w');
                simpl in Heqn; rewrite Heqb in Heqn; simpl in Heqn
-           end.
+           end. *)
 Qed.
 
 Lemma NToWord_zero {sz} :
@@ -1022,7 +1023,7 @@ Proof.
     try solve [split; reflexivity];
     try solve [match goal with
                | [ H: _ \/ _ |- _ ] => destruct H; try congruence
-               end].
+               end];
   first [apply combine_inj; eassumption
         | solve [intuition] ].
 Qed.
